helpers.v
@@ -251,9 +251,9 @@ Section Histories.
         |rewrite <- Nat.eqb_neq in *; rewrite n in *]; auto.
       eapply IHgenerated.
       rewrite <- Heqs1ycpy. apply in_or_app; left; auto.
-    - unfold get_emulate_response in *.
-      functional induction (get_emulate_response_helper
-                              (state_with_md s1 Emulate) t i 0);
+    - unfold get_oracle_response in *.
+      functional induction (get_oracle_response_helper
+                              (state_with_md s1 Oracle) t i 0);
         inversion H; subst; auto.
     - destruct (rev (X_copy s1));
         unfold get_replay_response, state_with_md in *; simpl in *;
@@ -280,9 +280,9 @@ Section Histories.
         [rewrite Nat.eqb_refl in *; rewrite rev_involutive in *
         |rewrite <- Nat.eqb_neq in *; rewrite n in *]; auto.
       apply in_inv in H2. destruct H2; [inversion H2; subst|]; auto.
-    - unfold get_emulate_response in *.
-      functional induction (get_emulate_response_helper
-                              (state_with_md s1 Emulate) t i 0);
+    - unfold get_oracle_response in *.
+      functional induction (get_oracle_response_helper
+                              (state_with_md s1 Oracle) t i 0);
         inversion H; subst; auto.
     - destruct (rev (X_copy s1));
         unfold get_replay_response, state_with_md in *; simpl in *;
@@ -348,7 +348,7 @@ Section Misc.
   Hint Resolve commH_state y_copy_state.
   
   Lemma next_mode_dec : forall s t i, {next_mode s t i = Commute}
-                                      + {next_mode s t i = Emulate}
+                                      + {next_mode s t i = Oracle}
                                       + {next_mode s t i = Replay}.
   Proof.
     intros; destruct s; unfold next_mode in *; simpl in *; destruct md.
@@ -525,15 +525,15 @@ Section Misc.
           eapply i0; eauto.
           eapply i1; eauto.
           rewrite <- Heqs1ycpy. apply in_or_app; left; auto.
-      + unfold get_emulate_response in *.
-        functional induction (get_emulate_response_helper
+      + unfold get_oracle_response in *.
+        functional induction (get_oracle_response_helper
          {|
          X_copy := X_copy s1;
          Y_copy := Y_copy s1;
          preH := preH s1;
          commH := commH s1;
          postH := postH s1;
-         md := Emulate |} t i 0); inversion H2; subst; simpl in *; auto.
+         md := Oracle |} t i 0); inversion H2; subst; simpl in *; auto.
       + remember (rev (X_copy s1)) as rxcpys1.
         destruct (rxcpys1); unfold get_replay_response in *; simpl in *; inversion H2; subst; auto.
         rewrite <- Heqrxcpys1 in *.
@@ -611,8 +611,8 @@ Section State_Lemmas.
           destruct (action_invocation_eq a t i); simpl in *; discriminate.
           destruct (rev (Y_copy s1 t));
             [discriminate | destruct (action_invocation_eq a t i); simpl in *; discriminate].
-        + unfold get_emulate_response in H.
-          functional induction (get_emulate_response_helper (state_with_md s1 Emulate) t0 i0 0);
+        + unfold get_oracle_response in H.
+          functional induction (get_oracle_response_helper (state_with_md s1 Oracle) t0 i0 0);
           inversion H; subst; simpl in *; auto.
         + unfold get_replay_response in H. remember (X_copy s1) as s1xcpy.
           destruct (s1xcpy).
@@ -643,9 +643,9 @@ Section State_Lemmas.
         destruct (rev (Y_copy (state_with_md s Commute) t));
         inversion Hact; subst;
         unfold state_with_md in *; simpl in *; auto; discriminate.
-      - unfold get_emulate_response in *.
-        functional induction (get_emulate_response_helper
-                                (state_with_md s Emulate) t i 0);
+      - unfold get_oracle_response in *.
+        functional induction (get_oracle_response_helper
+                                (state_with_md s Oracle) t i 0);
           unfold state_with_md in *; simpl in *;
           inversion Hact; subst; simpl in *; try discriminate.
         now apply IHp.
@@ -677,9 +677,9 @@ Section State_Lemmas.
            destruct (next_mode s1 t i); auto.
            - unfold get_commute_response in *; unfold state_with_md in *; simpl in *.
              destruct (rev (Y_copy s1 t)) in *; inversion H1; subst; discriminate.
-           - unfold get_emulate_response in *.
-             functional induction (get_emulate_response_helper
-                                     (state_with_md s1 Emulate) t i 0);
+           - unfold get_oracle_response in *.
+             functional induction (get_oracle_response_helper
+                                     (state_with_md s1 Oracle) t i 0);
                inversion H1; subst; try discriminate.
              now eapply IHp.
          }
@@ -766,9 +766,9 @@ Section State_Lemmas.
           destruct (rev (Y_copy s1 t)); try discriminate.
           destruct (action_invocation_eq a t i); try discriminate.
           now right. now left. now right.
-          unfold get_emulate_response in *.
-          functional induction (get_emulate_response_helper
-                                  (state_with_md s1 Emulate) t i 0);
+          unfold get_oracle_response in *.
+          functional induction (get_oracle_response_helper
+                                  (state_with_md s1 Oracle) t i 0);
             inversion H1; subst; simpl in *; try discriminate.
           eapply IHp; eauto.
           now left. now right. now left.
@@ -793,15 +793,15 @@ Section State_Lemmas.
             {
               remember (action_invocation_eq x t i) as Hacteq.
               destruct Hacteq; auto. 
-              unfold get_emulate_response, state_with_md in *; simpl in *.
-              functional induction (get_emulate_response_helper
+              unfold get_oracle_response, state_with_md in *; simpl in *.
+              functional induction (get_oracle_response_helper
                                       {|
                                         X_copy := HX ++ [x];
                                         Y_copy := history_of_thread Y;
                                         preH := [];
                                         commH := fun _ : tid => [];
                                         postH := [];
-                                        md := Emulate |} t i 0);
+                                        md := Oracle |} t i 0);
                 inversion H1; subst; try discriminate.
               now eapply IHp.
             }
@@ -827,15 +827,15 @@ Section State_Lemmas.
                 unfold next_mode in *; remember (md s1) as s1md; destruct s1md; try discriminate.
               destruct (rev (X_copy s1)); try discriminate. destruct (action_invocation_eq a t i);
                                                               discriminate.
-              unfold get_emulate_response, state_with_md in *; simpl in *. clear H8.
-              functional induction (get_emulate_response_helper
+              unfold get_oracle_response, state_with_md in *; simpl in *. clear H8.
+              functional induction (get_oracle_response_helper
                                       {|
                                         X_copy := X_copy s1;
                                         Y_copy := Y_copy s1;
                                         preH := preH s1;
                                         commH := commH s1;
                                         postH := postH s1;
-                                        md := Emulate |} t i 0);
+                                        md := Oracle |} t i 0);
                 inversion H1; subst; try discriminate.
               now eapply IHp.
 
@@ -855,13 +855,13 @@ Section State_Lemmas.
               destruct (Nat.eq_dec is1 i), (Nat.eq_dec t ts1); subst;
                 repeat try rewrite Nat.eqb_refl in *; try rewrite <- Nat.eqb_neq in *;
                   try rewrite n in *; try rewrite n0 in *; simpl in *; auto.
-              all: unfold get_emulate_response in *.
-              1,3: functional induction (get_emulate_response_helper
-                                        (state_with_md s1 Emulate) t (Inv i) 0);
+              all: unfold get_oracle_response in *.
+              1,3: functional induction (get_oracle_response_helper
+                                        (state_with_md s1 Oracle) t (Inv i) 0);
                 inversion H1; subst; unfold state_with_md in *; simpl in *; try discriminate;
                   try now eapply IHp.
-              functional induction (get_emulate_response_helper
-                                        (state_with_md s1 Emulate) ts1 (Inv i) 0);
+              functional induction (get_oracle_response_helper
+                                        (state_with_md s1 Oracle) ts1 (Inv i) 0);
                 inversion H1; subst; unfold state_with_md in *; simpl in *; try discriminate;
                   try now eapply IHp.
             }
@@ -884,9 +884,9 @@ Section State_Lemmas.
           destruct s1ycpy using rev_ind; simpl in *; try rewrite rev_unit in *;
             [| destruct (action_invocation_eq x t i)].
           
-          1,3: unfold get_emulate_response in *;
-            functional induction (get_emulate_response_helper
-                                    (state_with_md s1 Emulate) t i 0);
+          1,3: unfold get_oracle_response in *;
+            functional induction (get_oracle_response_helper
+                                    (state_with_md s1 Oracle) t i 0);
             inversion H1; subst; unfold state_with_md in *; simpl in *; try discriminate;
               try now eapply IHp.
 
@@ -914,33 +914,33 @@ Section State_Lemmas.
           eapply i0; eauto.
     Qed.
 
-  Lemma not_emulate_postH_nil :
+  Lemma not_oracle_postH_nil :
     forall h s,
       generated s h ->
-      s.(md) <> Emulate ->
+      s.(md) <> Oracle ->
       s.(postH) = [].
     Proof.
       induction h; intros; inversion H; subst.
       unfold start_state in *; simpl in *; auto.
-      assert (s1.(md) <> Emulate).
+      assert (s1.(md) <> Oracle).
       {
         unfold emulator_act in *.
         unfold next_mode in *.
         remember (md s1) as mds1. destruct mds1; subst; try discriminate.
-        unfold get_emulate_response in *.
-        functional induction (get_emulate_response_helper
-                                (state_with_md s1 Emulate) t i 0);
+        unfold get_oracle_response in *.
+        functional induction (get_oracle_response_helper
+                                (state_with_md s1 Oracle) t i 0);
           inversion H3; subst; auto.
       }
       pose (IHh s1 H6 H1).
       unfold emulator_act in *.
-      assert (next_mode s1 t i <> Emulate).
+      assert (next_mode s1 t i <> Oracle).
       {
         unfold emulator_act in *.
         remember (next_mode s1 t i) as mds1. destruct mds1; subst; try discriminate.
-        unfold get_emulate_response in *.
-        functional induction (get_emulate_response_helper
-                                (state_with_md s1 Emulate) t i 0);
+        unfold get_oracle_response in *.
+        functional induction (get_oracle_response_helper
+                                (state_with_md s1 Oracle) t i 0);
           inversion H3; subst; auto.
       }
       remember (next_mode s1 t i) as s1nextmd.
@@ -953,16 +953,16 @@ Section State_Lemmas.
       destruct xcpy; rewrite <- Heqxcpy in *; simpl in *; inversion H3; subst; auto.
     Qed.
     
-  Lemma emulate_response_state :
+  Lemma oracle_response_state :
     forall h s t i s' a,
       generated s h ->
       spec ((t,i,NoResp) :: h) ->
-      get_emulate_response (state_with_md s Emulate) t i = (s', a) ->
+      get_oracle_response (state_with_md s Oracle) t i = (s', a) ->
       s.(commH) = s'.(commH) /\ s'.(postH) = a :: s.(postH) /\ s'.(preH) = s.(preH).
   Proof.
     intros.
-    unfold get_emulate_response in *; simpl in *.
-    functional induction (get_emulate_response_helper (state_with_md s Emulate)
+    unfold get_oracle_response in *; simpl in *.
+    functional induction (get_oracle_response_helper (state_with_md s Oracle)
                                                       t i 0);
       unfold state_with_md in *; simpl in *;
         inversion H1; subst; auto.
@@ -989,8 +989,8 @@ Section State_Lemmas.
         destruct (action_invocation_eq a t i); discriminate.
         destruct (rev (Y_copy s1 t)); [|destruct (action_invocation_eq a t i)]; discriminate.
         destruct (rev (Y_copy s1 t)); [|destruct (action_invocation_eq a0 t i)]; discriminate.
-      - unfold get_emulate_response in *.
-        functional induction (get_emulate_response_helper (state_with_md s1 Emulate)
+      - unfold get_oracle_response in *.
+        functional induction (get_oracle_response_helper (state_with_md s1 Oracle)
                                                           t0 i0 0);
           unfold next_mode in H1; inversion H4; subst; simpl in *; auto.
     }
@@ -1047,16 +1047,16 @@ Section State_Lemmas.
                [rewrite Nat.eqb_refl in *| rewrite <- Nat.eqb_neq in *; rewrite n in *].
              inversion H1; subst; auto. eapply i0; eauto.
           -- assert (postH s1 = []).
-             eapply not_emulate_postH_nil; eauto.
+             eapply not_oracle_postH_nil; eauto.
              unfold next_mode in Heqs1nmd.
              remember (md s1) as s1md. destruct s1md; try discriminate.
              rewrite H1 in *; simpl in *; auto.
       + exists gencomm.
         split; auto.
-        -- assert (commH s1 = commH s). eapply emulate_response_state; eauto.
+        -- assert (commH s1 = commH s). eapply oracle_response_state; eauto.
            rewrite <- H3. auto.
         -- assert (postH s = (t,i,r) :: postH s1 /\ preH s = preH s1).
-           eapply emulate_response_state; eauto.
+           eapply oracle_response_state; eauto.
            destruct_conjs; subst.
            rewrite H3, H6; simpl in *; auto.
       + exists gencomm.
@@ -1196,7 +1196,7 @@ Section State_Lemmas.
               unfold get_commute_response in *. rewrite H3 in *. inversion H2; subst; auto.
             }
             eapply during_commute_state; eauto.
-          * pose (emulate_response_state _ _ _ _ _ _ H5 H4 H2).
+          * pose (oracle_response_state _ _ _ _ _ _ H5 H4 H2).
             destruct_conjs.
             rewrite H6. auto.
           * assert (md s1 = Replay).
@@ -1220,7 +1220,7 @@ Section State_Lemmas.
               unfold get_commute_response in *. rewrite H6 in *. inversion H2; subst; auto.
             }
             left; eapply during_commute_state; eauto.
-          * pose (emulate_response_state _ _ _ _ _ _ H5 H4 H2).
+          * pose (oracle_response_state _ _ _ _ _ _ H5 H4 H2).
             destruct_conjs.
             rewrite H6, H3. auto. rewrite H0.
             right; split; simpl; auto.
